getting ready to prove main thms for multiplier

src/multiplier.v
@@ -96,7 +96,7 @@ Module Basic.
      then shift-right by one by reassembly. *)
   Definition shift_and_add (b : bv 4) (a : bv 8) : bv 8 :=
     let t0 := bv_extract 4 5 a in
-    let t1 := if bv_odd a then bv_zero_extend 5 b else 0 in
+    let t1 := if bv_odd a then 5#b else 0 in
     bv_concat 8 (t0 + t1) (bv_extract 1 3 a).
 
   Definition cycle (s : State) (inp : In) : State * Out :=
@@ -104,7 +104,7 @@ Module Basic.
     then
       if inp.(InValid) =? 1
       then
-        let ra' := bv_zero_extend 8 inp.(InA) in
+        let ra' := 8#inp.(InA) in
         let rb' := inp.(InB) in
         let rcount' := 3 in
         let rbusy' := 1 in
@@ -143,7 +143,7 @@ Module Basic.
     | i :: ins' =>
         let (s', out) := cycle s i in
         let (s'', outs) := cycles s' ins' in
-        (s', out :: outs)
+        (s'', out :: outs)
     end.
 
   Fixpoint repeat {A : Type} (f : A -> A) (n : nat) {struct n} : (A -> A) :=
@@ -196,7 +196,7 @@ Module Basic.
   Ltac case_range16 :=
     repeat match goal with
       | [ H : (0 <= ?z < 16)%Z |- _ ] =>
-          let Hz := fresh "H_cases" in
+          let Hz := fresh "Hcases" in
           assert (z = 0 \/ z = 1 \/ z = 2 \/ z = 3 \/ z = 4 \/ z = 5 \/ z = 6 \/ z = 7 \/
                     z = 8 \/ z = 9 \/ z = 10 \/ z = 11 \/ z = 12 \/ z = 13 \/ z = 14 \/ z = 15)%Z
             as Hz by lia; clear H;
@@ -215,12 +215,29 @@ Module Basic.
   Qed.
 
   Lemma shift_and_add4_multiplies : forall (a b : bv 4),
-      bv_unsigned (shift_and_add4 b (bv_zero_extend 8 a)) = (bv_unsigned a * bv_unsigned b)%Z.
+      bv_unsigned (shift_and_add4 b (8#a)) = (bv_unsigned a * bv_unsigned b)%Z.
   Proof.
     intros a b. rewrite <- shift_and_add4_equiv.
-    Search bv_unsigned bv_zero_extend. rewrite bv_zero_extend_unsigned.
+    Search bv_unsigned bv_zero_extend. rewrite bv_zero_extend_unsigned by lia.
     apply shift_and_add4'_multiplies. all: bv_solve.
   Qed.
+
+  Notation "a *| b" := ((8#a) * (8#b)) (at level 35).
+
+  Lemma shift_and_add4_correct : forall (a b : bv 4),
+      shift_and_add4 b (8#a) = a *| b.
+  Proof.
+    intros a b. Search (bv_unsigned _ = bv_unsigned _).
+    rewrite bv_eq. Search bv_mul.
+    rewrite bv_mul_unsigned.
+    Search bv_zero_extend bv_unsigned.
+    repeat rewrite bv_zero_extend_unsigned by lia.
+    Check bv_wrap_small. rewrite bv_wrap_small.
+    apply shift_and_add4_multiplies. bv_saturate_unsigned.
+    unfold bv_modulus in *; simpl in *. nia.
+  Qed.
+
+  Hint Resolve shift_and_add4_correct : multiplier.
 
   Lemma bv1_is_0_or_1 : forall (b : bv 1), b = 0 \/ b = 1.
   Proof.
@@ -240,60 +257,150 @@ Module Basic.
          | |- ?b = 1 :> bv 1 => pose proof (bv1_is_0_or_1 b); intuition
          end : multiplier.
 
-  Lemma cycle_idle_valid : forall s s' a b i o,
-      ~ busy s -> valid i -> a = i.(InA) -> b = i.(InB) -> (s', o) = cycle s i ->
-      s' = s <| R := {| RA := 8#a; RB := b; RCount := 3; RBusy := 1 |} |>
-             <| T := s.(T) ++ [{| LeakValid := 1; LeakReady := 0 |}] |>
-       /\ o = Out0.
+  Definition cycle_idle_valid s1 i s2 o : Prop := forall a b,
+      ~ busy s1 -> valid i -> a = i.(InA) -> b = i.(InB) -> (s2, o) = cycle s1 i ->
+      s2 = s1 <| R := {| RA := 8#a; RB := b; RCount := 3; RBusy := 1 |} |>
+              <| T := s1.(T) ++ [{| LeakValid := 1; LeakReady := 0 |}] |>
+      /\ o = Out0.
+
+  Lemma cycle_idle_valid_holds : forall s1 i s2 o, cycle_idle_valid s1 i s2 o.
   Proof.
+    unfold cycle_idle_valid.
     repeat progress (intros; simpl; subst).
     unfold cycle in *. unfold bv_eqb in *. unfold busy in *.
-    unfold valid in *. assert (s.(R).(RBusy) = 0) by auto with multiplier.
+    unfold valid in *. assert (s1.(R).(RBusy) = 0) by auto with multiplier.
     repeat rewrite H1 in H3. simpl in *. rewrite H0 in H3.
     simpl in *. inversion H3; clear H3. subst. done.
   Qed.
 
-  Lemma cycle_idle_invalid : forall s s' i o,
-      ~ busy s -> ~ valid i -> (s', o) = cycle s i ->
-      s' = s <| T := s.(T) ++  [{| LeakValid := 0; LeakReady := 0 |}] |>
-      /\ o = Out0.
+  Hint Resolve cycle_idle_valid_holds : multiplier.
+
+  Definition cycle_idle_invalid s1 i s2 o : Prop :=
+    ~ busy s1 -> ~ valid i -> (s2, o) = cycle s1 i ->
+    s2 = s1 <| T := s1.(T) ++  [{| LeakValid := 0; LeakReady := 0 |}] |>
+    /\ o = Out0.
+
+  Lemma cycle_idle_invalid_holds : forall s1 i s2 o, cycle_idle_invalid s1 i s2 o.
   Proof.
+    unfold cycle_idle_invalid.
     repeat progress (intros; simpl; subst).
     unfold cycle, bv_eqb, busy, valid in *.
-    assert (s.(R).(RBusy) = 0) by auto with multiplier.
+    assert (s1.(R).(RBusy) = 0) by auto with multiplier.
     assert (i.(InValid) = 0) by auto with multiplier.
     rewrite H2, H3 in H1. simpl in *. inversion H1; clear H1.
     done.
   Qed.
 
-  Lemma cycle_busy_unfinished : forall s s' i o,
-      busy s -> ~ finished s -> (s', o) = cycle s i ->
-      s' = s <| R; RA := shift_and_add s.(R).(RB) s.(R).(RA) |>
-             <| R; RCount := s.(R).(RCount) - 1 |>
-             <| T := s.(T) ++ [{| LeakValid := i.(InValid); LeakReady := 0 |}] |>
+  Hint Resolve cycle_idle_invalid_holds : multiplier.
+
+  Definition cycle_busy_unfinished s1 i s2 o : Prop :=
+    busy s1 -> ~ finished s1 -> (s2, o) = cycle s1 i ->
+      s2 = s1 <| R; RA := shift_and_add s1.(R).(RB) s1.(R).(RA) |>
+              <| R; RCount := s1.(R).(RCount) - 1 |>
+              <| T := s1.(T) ++ [{| LeakValid := i.(InValid); LeakReady := 0 |}] |>
       /\ o = Out0.
+
+  Lemma cycle_busy_unfinished_holds : forall s1 i s2 o, cycle_busy_unfinished s1 i s2 o.
   Proof.
+    unfold cycle_busy_unfinished.
     repeat progress (intros; simpl; subst).
     unfold cycle, bv_eqb, busy, finished in *.
     rewrite H in H1; simpl in *.
-    destruct (bv_eq_dec 2 (RCount (R s)) 0) as [Heq | Hneq].
+    destruct (bv_eq_dec 2 (RCount (R s1)) 0) as [Heq | Hneq].
     - done.
     - inversion H1; clear H1; subst. intuition congruence.
   Qed.
 
-  Lemma cycle_busy_finished : forall s s' i o,
-      busy s -> finished s -> (s', o) = cycle s i ->
-      s' = s <| R; RA := shift_and_add s.(R).(RB) s.(R).(RA) |>
-             <| R; RCount := 0 |>
-             <| R; RBusy := 0 |>
-             <| T := s.(T) ++ [{| LeakValid := i.(InValid); LeakReady := 1 |}] |>
-      /\ o = {| OutP := s'.(R).(RA); OutReady := 1 |}.
+  Hint Resolve cycle_busy_unfinished_holds : multiplier.
+
+  Definition cycle_busy_finished s1 i s2 o : Prop :=
+    busy s1 -> finished s1 -> (s2, o) = cycle s1 i ->
+      s2 = s1 <| R; RA := shift_and_add s1.(R).(RB) s1.(R).(RA) |>
+              <| R; RCount := 0 |>
+              <| R; RBusy := 0 |>
+              <| T := s1.(T) ++ [{| LeakValid := i.(InValid); LeakReady := 1 |}] |>
+      /\ o = {| OutP := s2.(R).(RA); OutReady := 1 |}.
+
+  Lemma cycle_busy_finished_holds : forall s1 i s2 o, cycle_busy_finished s1 i s2 o.
   Proof.
+    unfold cycle_busy_finished.
     repeat progress (intros; simpl; subst).
     unfold cycle, bv_eqb, busy, finished in *.
     rewrite H in H1; simpl in *. rewrite H0 in H1.
     simpl in *. inversion H1; clear H1; subst. done.
   Qed.
+
+  Hint Resolve cycle_busy_finished_holds : multiplier.
+
+  Inductive cycle_spec : State -> In -> State -> Out -> Prop :=
+    | CycleIdleValid : forall s1 i s2 o,
+        cycle_idle_valid s1 i s2 o -> cycle_spec s1 i s2 o
+    | CycleIdleInvalid : forall s1 i s2 o,
+        cycle_idle_invalid s1 i s2 o -> cycle_spec s1 i s2 o
+    | CycleBusyUnfinished : forall s1 i s2 o,
+        cycle_busy_unfinished s1 i s2 o -> cycle_spec s1 i s2 o
+    | CycleBusyFinished : forall s1 i s2 o,
+        cycle_busy_finished s1 i s2 o -> cycle_spec s1 i s2 o.
+
+  Hint Constructors cycle_spec : multiplier.
+
+  (* We state the theorem that we can use the inductive proposition given
+     that we have the Gallina function. *)
+  Theorem cycle_complete : forall s1 i s2 o,
+      (s2, o) = cycle s1 i -> cycle_spec s1 i s2 o.
+  Proof.
+    intros s1 i s2 o Hcycle. unfold cycle in *.
+    destruct (s1.(R).(RBusy) =? 0) as [|].
+    - destruct (i.(InValid) =? 1) as [|].
+      + inversion Hcycle; clear Hcycle; subst.
+        constructor; apply cycle_idle_valid_holds.
+      + inversion Hcycle; clear Hcycle; subst.
+        constructor; apply cycle_idle_invalid_holds.
+    - destruct (s1.(R).(RCount) =? 0) as [|].
+      + inversion Hcycle; clear Hcycle; subst.
+        constructor; apply cycle_busy_unfinished_holds.
+      + inversion Hcycle; clear Hcycle; subst.
+        constructor; apply cycle_busy_finished_holds.
+  Qed.
+
+  Inductive cycles_spec : State -> list In -> State -> list Out -> Prop :=
+    | CyclesRefl : forall s, cycles_spec s [] s []
+    | CyclesTrans : forall s i s' (o : Out) is s'' o os,
+        cycle_spec s i s' o ->
+        cycles_spec s' is s'' os ->
+        cycles_spec s (i :: is) s'' (o :: os).
+
+  Hint Constructors cycles_spec : multiplier.
+
+  Lemma cycles_complete' : forall is s1 s2 os,
+      (s2, os) = cycles s1 is -> cycles_spec s1 is s2 os.
+  Proof.
+    intro is. induction is; intros.
+    - simpl in *. inversion H. constructor.
+    - simpl in *. case_match. case_match. inversion H. subst.
+      clear H. apply CyclesTrans with (s' := s).
+      + done.
+      + apply cycle_complete. symmetry. assumption.
+      + apply IHis. symmetry. assumption.
+  Qed.
+
+  Theorem cycles_complete : forall s1 is s2 os,
+      (s2, os) = cycles s1 is -> cycles_spec s1 is s2 os.
+  Proof.
+    intros s1 is s2 os. exact (cycles_complete' is s1 s2 os).
+  Qed.
+
+  (* Finally, with all those helper theorems out of the way, we can now prove
+     the following correctness property:
+
+     For any cycle where the circuit is idle, if a valid [a] and [b] are
+     provided, four cycles later it will produce [a *| b]. *)
+  Theorem cycles_correct : forall s1 s2 i1 i2 i3 i4 os a b,
+      ~ busy s1 -> i1 = {| InA := a; InB := b; InValid := 1 |} ->
+      (s2, os) = cycles s1 [i1; i2; i3; i4] ->
+      os = [Out0; Out0; Out0; {| OutP := a *| b; OutReady := 1 |}].
+  Admitted.
+
 
   (** NOTE knwabueze for aerbsen: I think we talked about using this definition
       for the extraction from the list of inputs to the specification leakage.
@@ -314,7 +421,7 @@ Module Basic.
   Definition extract : list In -> list SLeakage :=
     map (fun i => if i.(InValid) =? 1 then Some i.(InA) else None).
 
-  Theorem ct : exists (predictor : list SLeakage -> list ILeakage),
+  Theorem cycle_ct : exists (predictor : list SLeakage -> list ILeakage),
     forall (s' : State) (is : list In) (os : list Out),
       (s', os) = cycles State0 is -> s'.(T) = (predictor ∘ extract) is.
   Admitted.
