src/bitvector.v
@@ -11,14 +11,10 @@ Section WithContext.
     Eval cbv beta iota zeta delta [ bool_decide decide_rel ] in
       bool_decide (x = y).
 
-  Definition bv_testbit (x : bv n) (i : Z) : bool :=
-    Z.testbit (bv_unsigned x) i.
-
   Definition bv_odd (x : bv n) := Z.odd (bv_unsigned x).
 End WithContext.
 
 
 Infix "=?" := bv_eqb (only parsing) : bv_scope.
-Infix "#" := bv_zero_extend (at level 35, only parsing) : bv_scope.
+Infix "#" := bv_zero_extend (at level 65, only parsing) : bv_scope.
 Infix "||" := (bv_concat _) (only parsing) : bv_scope.
-Infix "!" := bv_testbit (at level 35, only parsing) : bv_scope.
